MetaTools/MetaTools.BrowseTerm.Tests.fst
@@ -1,0 +1,46 @@
+module MetaTools.BrowseTerm.Tests
+
+open FStar.Tactics
+open Control.Monoid
+
+open FStar.Tactics.Typeclasses
+open MetaTools.Util
+open MetaTools.BrowseTerm
+
+module L = FStar.List.Tot
+
+let rebuiltTopLevel_works t: Tac term = 
+  fst
+  (browse_term #unit #unitIsMonoid
+    (fun beforeTransform rebuildToplevel boundedVariables parents currentTerm -> 
+      (( if beforeTransform
+        then currentTerm
+        else (
+           let rebuilt = rebuildToplevel currentTerm in
+           let strict = compare_term rebuilt t = FStar.Order.Eq in
+           let relaxed = term_to_string rebuilt = term_to_string t in 
+           ( if relaxed
+             then ()
+             else dump (
+                      "(Err rebuiltTopLevel_works)\n## Child\n"
+                    ^ term_to_string currentTerm
+                    ^ "\n\n## Toplevel\n"
+                    ^ term_to_string rebuilt
+                    ^ "\n\n## Actual toplevel\n"
+                    ^ term_to_string t
+                    ^ "\n\n## Parents\n"
+                    ^ term_heads_to_string parents
+                  )
+           );
+           currentTerm
+        )
+      ), id_tac), ()
+    )
+    t)
+
+
+let _: unit = _ by (
+  let _ = rebuiltTopLevel_works (`(fun x y -> x + y + 4)) in
+  exact (`())
+)
+
