MetaTools/MetaTools.Erase.fst
@@ -7,39 +7,52 @@ module U = MetaTools.Util
 module L = FStar.List.Tot
 
 open FStar.Tactics
+open Control.Monoid
 
+[@plugin]
 let typechecks (t: term): Tac bool
-  = Some? (trytac (fun _ -> tc (top_env ()) t))
+  = Some? (trytac (fun _ -> tc t))
 
-
-type label =
-type labeled (a: Type) =
+type label = int
+type labeled (a: Type) = label * a
 
 assume val placeholder: (#a: Type) -> a
 
-let erase #a (v: labeled a) (at: label): labeled a
-  = placeholder
+let erase a (v: labeled a) (at: label): labeled a
+  = if at > fst v
+    then placeholder
+    else v
 
 let erase_term_helper
   (eraseVarParam: term)
   (rebuildToplevel: term -> Tac term)
   (t: term)
-  = let erased_t = pack (Tv_App (`erase) (t, Q_Explicit)) in
-    if typechecks erased_t
-    then erased_t
-    else t
+  : Tac (term * (term -> Tac term))
+  = let do_erase t: Tac term = mk_app (`erase)
+      [ pack Tv_Unknown, Q_Explicit
+      ; t, Q_Explicit
+      ; eraseVarParam, Q_Explicit
+      ] in
+    let toplevel_erased = rebuildToplevel (do_erase t) in
+    let log m =
+      dump (term_to_string t ^ "\n" ^ term_to_string toplevel_erased ^ "\nRESPONSE:"^m)
+    in
+    if typechecks (rebuildToplevel t)//toplevel_erased
+    then (log "YES"; t, do_erase)
+    else (log "NOP"; t, id_tac)
 
 let erase_term (eraseVarParam t: term): Tac term = 
   fst
-  (browse_term #unit
+  (browse_term #unit #unitIsMonoid
     (fun beforeTransform rebuildToplevel boundedVariables parents currentTerm -> 
-      ( if beforeTransform
-        then erase_term_helper eraseVarParam rebuildToplevel currentTerm
-        else currentTerm
+      ( if (beforeTransform = false)
+        then currentTerm, id_tac
+        else (
+          erase_term_helper eraseVarParam rebuildToplevel currentTerm
+        )
       ), ()
     )
     t)
-
 
 let blacklist_lioCore (n: name) =
   match n with
@@ -49,36 +62,47 @@ let blacklist_lioCore (n: name) =
   | "Prims"::_ -> true
   | _ -> false
 
-let bv_erase = "cur_label_name_GLOBAL"
-
-open FStar.Tactics.Typeclasses
-
-
-let replace_fv (t: term) (r: list (name * name))
+let replace_fv (t: term) (r: list (name * term))
   : Tac term
-  = fst (browse_term #unit begin
+  = fst (browse_term #unit #unitIsMonoid begin
     fun beforeTransform _ _ _ currentTerm
-    -> ( if beforeTransform
+    -> ((if beforeTransform
         then begin
              match inspect currentTerm with
              | Tv_FVar fv ->
                let n = inspect_fv fv in
                ( match L.find (fun (old, _) -> old = n) r with
-               | Some (_, newName) -> pack (Tv_FVar (pack_fv newName))
+               | Some (_, replaceTerm) -> replaceTerm
                | _ -> currentTerm
                )
              | _ -> currentTerm
              end
-        else currentTerm ), ()
+        else currentTerm ), id_tac), ()
   end t)
 
 let make_erased_name (n: name): Tac name =
-  cur_module () @ [last n ^ "_erased"]
+  guard (Cons? n);
+  cur_module () @ [U.last n ^ "_erased"]
 
-let make_erased_names (n: list name): Tac (list (_ * _))
-  = map (fun n -> n, make_erased_name n) n
+let make_erased_replacements (lvar: bv) (n: list name): Tac (list (name * term))
+  = map (fun n ->
+    n, (
+      let t = pack (Tv_FVar (pack_fv (make_erased_name n))) in
+      mk_app t [pack (Tv_Var lvar), Q_Explicit]
+    )
+  ) n
 
+module Typeclasses = FStar.Tactics.Typeclasses
+
+let rec zip #a (l: list a) #b (r: list b)
+  : list (a * b)
+  = match l, r with
+  | hl::tl, hr::tr -> (hl, hr)::zip tl tr
+  | _ -> []
+
+let bv_erase = "cur_label_name_GLOBAL"
 let erase_term_and_defs (def: term)
+ : Tac (list (name * option (term * term)))
   =
     let label_var: bv = pack_bv ({
         bv_ppname = bv_erase;
@@ -93,14 +117,57 @@ let erase_term_and_defs (def: term)
     in
     let h arg: Tac (option (term * term)) =
       let toplevel_name, dependencies = arg in
-      let replacements = make_erased_names dependencies in
-      let patch t: Tac term = replace_fv t replacements in
-      U.optmap (fun (typ, def)
-        -> 
-          let b_lvar = fresh_binder (`label) in
+      let replacements = make_erased_replacements label_var dependencies in
+      let patch (t: term): Tac term = replace_fv t replacements in
+      match U.sglet_of_name toplevel_name with
+      | Some (typ, def) ->
+         Some (
+          let b_lvar: binder = fresh_binder (`label) in
           mk_tot_arr [b_lvar] (patch (erase_term (binder_to_term b_lvar) typ))
-        , mk_abs [pack_binder label_var Q_Explicit] (patch (erase_term label_var_term def))
-      ) (U.sglet_of_name toplevel_name)
+        , (
+          Typeclasses.mk_abs
+            [pack_binder label_var Q_Explicit]
+            (patch (erase_term label_var_term def))
+          )
+        )
+      | None -> None
+      // U.optmap (fun (typ, def)
+      //   -> 
+      //     let b_lvar = fresh_binder (`label) in
+      //     mk_tot_arr [b_lvar] (patch (erase_term (binder_to_term b_lvar) typ))
+      //   , Typeclasses.mk_abs [pack_binder label_var Q_Explicit] (patch (erase_term label_var_term def))
+      // ) (U.sglet_of_name toplevel_name)
     in
-    map h g
+    zip (L.map fst g) (map h g)
+
+
+
+let valOf (x: labeled int): int = snd x 
+
+let add (x y: labeled int) = 
+  valOf x + valOf y
+
+let hey: (list (name * option (term * term)))
+  = _ by (
+    let x = erase_term_and_defs (`add) in
+    // let _ = typechecks (`(snd (1, 2))) in
+    exact (quote x)
+  )
+
+
+// let f n: normalize_term (if n then (int -> int) else (int -> int -> int))
+// = let c1: int -> int = magic ()
+  
+
+
+let _ = fun cur_label_name_GLOBAL x y ->
+  Prims.op_Addition (valOf (erase _ x cur_label_name_GLOBAL))
+    (valOf y)
     
+
+let _ = fun x y glb ->
+  Prims.op_Addition (valOf x)
+    (valOf (erase _ y glb))
+
+let xx x (y: labeled int)
+  = erase _ (FStar.Pervasives.Native.snd y) x
